Exercise #2:
Using call-by-value evaluation and then lazy evaluation, write out the
first 10 steps of the evaluation of the following:

take 2 (makefrom 4 5)

Use the following definitions (clearly not OCaml syntax):

   take n [] = []
   take 0 (x::xs) = []
   take n (x::xs) = x::take (n-1) xs

   makefrom 0 v = []
   makefrom n v = v :: makefrom (n-1) (v+1)

-- call by need / lazy evaluation
  take 2 (makefrom 4 5)
= take 2 (5 :: makefrom (4-1) (5+1))
= 5 :: take (2-1) (makefrom (4-1) (5+1))
= 5 :: take (2-1) (makefrom 3 (5+1))
= 5 :: take (2-1) (v1 :: makefrom (3-1) (v1+1))
  where v1 = 5+1
= 5 :: take 1 (v1 :: makefrom (3-1) (v1+1))
  where v1 = 5+1
= 5 :: v1 :: take (1-1) (makefrom (3-1) (v1+1))
  where v1 = 5+1
= 5 :: v1 :: take (1-1) (makefrom (3-1) (v1+1))
   where v1 = 6
= 5 :: 6 :: take (1-1) (makefrom (3-1) (6+1))
= 5 :: 6 :: take (1-1) (makefrom 2 (6+1))
= 5 :: 6 :: take (1-1) (v2 :: makefrom (2-1) (v2+1))
  where v2 = 6+1
= 5 :: 6 :: take 0 (v2 :: makefrom (2-1) (v2+1))
  where v2 = 6+1
= 5 :: 6 :: []

-- call by name
  take 2 (makefrom 4 5)
= take 2 (5 :: makefrom (4-1) (5+1))
= 5 :: take (2-1) (makefrom (4-1) (5+1))
= 5 :: take (2-1) (makefrom 3 (5+1))
= 5 :: take (2-1) ( (5+1) :: makefrom (3-1) ((5+1)+1))
= 5 :: take 1  ( (5+1) :: makefrom (3-1) ((5+1)+1))
= 5 :: (5+1) :: take (1-1) (makefrom (3-1) ((5+1)+1))
= 5 :: 6 :: take (1-1) (makefrom (3-1) ((5+1)+1))
= 5 :: 6 :: take (1-1) (((5+1)+1) :: makefrom (2-1) ((5+1)+1)+1))
= 5 :: 6 :: take 0 (((5+1)+1) :: makefrom (2-1) ((5+1)+1)+1))
= 5 :: 6 :: []

-- call by value 
  take 2 (makefrom 4 5)
= take 2 (5 :: makefrom (4-1) (5+1))
= take 2 (5 :: makefrom 3 (5+1))
= take 2 (5 :: makefrom 3 6)
= take 2 (5 :: 6 :: makefrom (3-1) (6+1))
= take 2 (5 :: 6 :: makefrom 2 (6+1))
= take 2 (5 :: 6 :: makefrom 2 7)
   .... stuff happen
= take 2 (5 :: 6 :: 7 :: 8 :: [])
= 5 :: take (2-1) (6::7::8::[])
= 5 :: take 1 (6::7::8::[])
= 5 :: 6 :: take (1-1) (7::8::[])
= 5 :: 6 :: take 0 (7::8::[])
= 5 :: 6 ::[]

